src/PFuncAbstractDomain.v
@@ -6,73 +6,70 @@ Local Open Scope string_scope.
 
 Section PFuncAbstractDomain.
 
-  Context {PFunc: eqType}
-          {PFI: PFuncImpl PFunc}.
+  Context {PMap PSet PwAff: eqType}
+          {PI: PresburgerImpl PMap PSet PwAff}.
 
   Definition concrete_state := prod_eqType RegisterMap RegisterMap.
 
-  Definition PFuncAD := @total_map_eqType string_eqType PFunc.
+  Definition PFuncMap := @total_map_eqType string_eqType (@PFunc_eqType PSet PwAff).
 
-  Definition bot_PFunc : PFuncAD :=
+  Definition bot_PFuncMap : PFuncMap :=
     (_ !-> constant_pfunc VBot).
 
-  Definition top_PFunc : PFuncAD :=
+  Definition top_PFuncMap : PFuncMap :=
     (_ !-> constant_pfunc VTop).
 
-  Definition join_PFunc (p1 p2: PFuncAD) :=
+  Definition join_PFuncMap (p1 p2: PFuncMap) :=
     t_pointwise_bin_op p1 p2 (fun x1 x2 => join_pfunc x1 x2).
 
-  Definition gamma_PFunc (p: PFuncAD) :=
+  Definition gamma_PFuncMap (p: PFuncMap) :=
     fun (x: concrete_state) => forall i, in_V (x.2 i) (eval_pfunc (p i) x.1).
 
-  Theorem gamma_top_PFunc :
-    forall x, Ensembles.In _ (gamma_PFunc top_PFunc) x.
+  Theorem gamma_top_PFuncMap :
+    forall x, Ensembles.In _ (gamma_PFuncMap top_PFuncMap) x.
   Proof.
-    move => x. rewrite /In /gamma_PFunc /top_PFunc => i /=.
+    move => x. rewrite /In /gamma_PFuncMap /top_PFuncMap.
     by auto_pfunc.
   Qed.
 
-  Theorem gamma_bot_PFunc :
-    forall x, ~ Ensembles.In _ (gamma_PFunc bot_PFunc) x.
+  Theorem gamma_bot_PFuncMap :
+    forall x, ~ Ensembles.In _ (gamma_PFuncMap bot_PFuncMap) x.
   Proof.
-    rewrite /In /gamma_PFunc /bot_PFunc => x /(_ "").
+    rewrite /In /gamma_PFuncMap /bot_PFuncMap => x /(_ "").
     by simpl_pfunc.
   Qed.
 
-  Theorem join_sound_l_PFunc :
-    forall a1 a2, Included _ (gamma_PFunc a1) (gamma_PFunc (join_PFunc a1 a2)).
+  Theorem join_sound_l_PFuncMap :
+    forall a1 a2, Included _ (gamma_PFuncMap a1) (gamma_PFuncMap (join_PFuncMap a1 a2)).
   Proof.
-    rewrite /Included /In /gamma_PFunc /join_PFunc => a1 a2 x Hle s.
-    move => /(_ s) in Hle. move: Hle.
-    simpl_pfunc.
+    rewrite /Included /In /gamma_PFuncMap /join_PFuncMap => a1 a2 x Hle s.
+    move => /(_ s) in Hle. move: Hle. simpl_pfunc.
     apply le_V_spec.
-    pose proof join_pfunc_spec_l.
-      by setoid_rewrite le_pfunc_spec in H.
+      by auto_pfunc.
   Qed.
 
-  Theorem join_sound_r_PFunc :
-    forall a1 a2, Included _ (gamma_PFunc a2) (gamma_PFunc (join_PFunc a1 a2)).
+  Theorem join_sound_r_PFuncMap :
+    forall a1 a2, Included _ (gamma_PFuncMap a2) (gamma_PFuncMap (join_PFuncMap a1 a2)).
   Proof.
-    rewrite /Included /In /gamma_PFunc /join_PFunc => a1 a2 x Hle s.
-    move => /(_ s) in Hle. move: Hle.
-    simpl_pfunc.
+    rewrite /Included /In /gamma_PFuncMap /join_PFuncMap => a1 a2 x Hle s.
+    move => /(_ s) in Hle. move: Hle. simpl_pfunc.
     apply le_V_spec.
-    pose proof join_pfunc_spec_r.
-      by setoid_rewrite le_pfunc_spec in H.
+    by auto_pfunc.
   Qed.
 
-  Instance adom_pmap : adom concrete_state PFuncAD :=
+  Instance adom_pmap : adom concrete_state PFuncMap :=
     {
-      bot := bot_PFunc;
-      top := top_PFunc;
-      join := join_PFunc;
+      bot := bot_PFuncMap;
+      top := top_PFuncMap;
+      join := join_PFuncMap;
 
-      gamma := gamma_PFunc;
+      gamma := gamma_PFuncMap;
 
-      gamma_top := gamma_top_PFunc;
-      gamma_bot := gamma_bot_PFunc;
-      join_sound_l := join_sound_l_PFunc;
-      join_sound_r := join_sound_r_PFunc;
+      gamma_top := gamma_top_PFuncMap;
+      gamma_bot := gamma_bot_PFuncMap;
+      join_sound_l := join_sound_l_PFuncMap;
+      join_sound_r := join_sound_r_PFuncMap;
     }.
+
 
 End PFuncAbstractDomain.
